a more precise spec in MasterSecret.derive

src/tls/MasterSecret.fst
@@ -12,7 +12,16 @@ module HH = FStar.HyperHeap
 
 type writer (ids:(AE.id * rid)) = w:AE.writer (fst ids){HH.extends (StreamAE.State.region w) (snd ids)}
 let ids = (AE.id * rid)
-let map_invariant (m:MM.map' ids writer) = True
+
+let region_exists (r:rid) = MR.witnessed (fun h -> Map.contains h r)
+    
+let map_invariant (m:MM.map' ids writer) =
+  forall i r. 
+    let wopt = MM.sel m (i, r) in
+    is_Some wopt ==>
+    HH.disjoint r tls_region 
+    /\ region_exists (StreamAE.State.region (Some.v wopt))
+
   (* Failed attempt *)
   (* (forall i1 i2. is_Some (m i1) /\ is_Some (m i2) /\ fst i1 = fst i2 ==> i1 = i2) *)
   (* /\ (forall i. is_None (m i) ==> (forall j. fst i = fst j ==> is_None (m j))) *)
@@ -22,19 +31,32 @@ let ms_tab : MM.t tls_region ids writer map_invariant =
 
 assume val gcut: f:(unit -> GTot Type){f()} -> Tot unit
 assume val gadmit: f:(unit -> GTot Type) -> Tot (u:unit{f()})
-
+assume val witness_rid: r:rid -> ST unit
+  (requires (fun h -> True))
+  (ensures (fun h0 _ h1 -> 
+	      h0 = h1 /\
+	      Map.contains h0 r /\
+	      region_exists r))
+	      
 let derive (r:rid) (i:AE.id) 
   : ST (AE.writer i)
        (requires (fun h -> disjoint r tls_region))
        (ensures (fun h0 w h1 -> 
 	   HH.extends (StreamAE.State.region w) r 
-	   /\ modifies (Set.singleton tls_region) h0 h1
-	   /\ MR.witnessed (MM.contains ms_tab (i,r) w)))
+	   /\ modifies (Set.singleton tls_region) h0 h1 //modifies at most the tls region
+	   /\ modifies_rref tls_region !{HH.as_ref (MR.as_rref ms_tab)} h0 h1 //and within it, at most ms_tab
+	   /\ MR.witnessed (MM.contains ms_tab (i,r) w) //and the writer is witnessed to be in ms_tab
+	   /\ (let old_ms = MR.m_sel h0 ms_tab in
+	      let new_ms = MR.m_sel h1 ms_tab in
+ 	       old_ms = new_ms //either ms_tab didn't change at all
+	       \/ (new_ms = MM.upd old_ms (i,r) w //or we just added w to it
+		  /\ (TLSInfo.authId i ==> MR.m_sel h1 (AE.ilog (StreamAE.State.log w)) = Seq.createEmpty))))) //and it is a fresh log
   = recall_region tls_region;
     let y = MM.lookup ms_tab (i, r) in
     match y with 
     | None -> 
       let w = AE.gen r i in 
+      witness_rid (StreamAE.State.region w);
       MM.extend ms_tab (i,r) w;
       w
     | Some w -> 
